Source/Dafny/Util.cs
@@ -2,6 +2,7 @@
 using System.Collections.Generic;
 using System.Linq;
 using System.Text;
+using System.Diagnostics.Contracts;
 
 using Microsoft.Boogie;
 
@@ -64,6 +65,100 @@ namespace Microsoft.Dafny {
         res[p.Item1] = p.Item2; 
       }
       return res;
+    }
+
+    /// <summary>
+    /// For "S" returns S and false.
+    /// For @"S" return S and true.
+    /// Assumes that s has one of these forms.
+    /// </summary>
+    public static string RemoveParsedStringQuotes(string s, out bool isVerbatimString) {
+      Contract.Requires(s != null);
+      var len = s.Length;
+      if (s[0] == '@') {
+        isVerbatimString = true;
+        return s.Substring(2, len - 3);
+      } else {
+        isVerbatimString = false;
+        return s.Substring(1, len - 2);
+      }
+    }
+    /// <summary>
+    /// Replaced any escaped characters in s by the actual character that the escaping represents.
+    /// Assumes s to be a well-parsed string.
+    /// </summary>
+    public static string RemoveEscaping(string s, bool isVerbatimString) {
+      Contract.Requires(s != null);
+      var sb = new StringBuilder();
+      UnescapedCharacters(s, isVerbatimString).Iter(ch => sb.Append(ch));
+      return sb.ToString();
+    }
+    /// <summary>
+    /// Returns the characters of the well-parsed string p, replacing any
+    /// escaped characters by the actual characters.
+    /// </summary>
+    public static IEnumerable<char> UnescapedCharacters(string p, bool isVerbatimString) {
+      Contract.Requires(p != null);
+      if (isVerbatimString) {
+        var skipNext = false;
+        foreach (var ch in p) {
+          if (skipNext) {
+            skipNext = false;
+          } else {
+            yield return ch;
+            if (ch == '"') {
+              skipNext = true;
+            }
+          }
+        }
+      } else {
+        var i = 0;
+        while (i < p.Length) {
+          char special = ' ';  // ' ' indicates not special
+          if (p[i] == '\\') {
+            switch (p[i + 1]) {
+              case '\'': special = '\''; break;
+              case '\"': special = '\"'; break;
+              case '\\': special = '\\'; break;
+              case '\0': special = '\0'; break;
+              case 'n': special = '\n'; break;
+              case 'r': special = '\r'; break;
+              case 't': special = '\t'; break;
+              case 'u':
+                int ch = HexValue(p[i + 1]);
+                ch = 16 * ch + HexValue(p[i + 2]);
+                ch = 16 * ch + HexValue(p[i + 3]);
+                ch = 16 * ch + HexValue(p[i + 4]);
+                yield return (char)ch;
+                i += 5;
+                continue;
+              default:
+                break;
+            }
+          }
+          if (special != ' ') {
+            yield return special;
+            i += 2;
+          } else {
+            yield return p[i];
+            i++;
+          }
+        }
+      }
+    }
+
+    /// <summary>
+    /// Converts a hexadecimal digit to an integer.
+    /// Assumes ch does represent a hexadecimal digit; alphabetic digits can be in either case.
+    /// </summary>
+    public static int HexValue(char ch) {
+      if ('a' <= ch && ch <= 'f') {
+        return ch - 'a' + 10;
+      } else if ('A' <= ch && ch <= 'F') {
+        return ch - 'A' + 10;
+      } else {
+        return ch - '0';
+      }
     }
 
   }
